theories/Reify/Patterns.v
@@ -1,4 +1,6 @@
-Definition table    (K V : Type) : Type := prod K V.
+Inductive table (K : Type) : Type := a_table.
+Inductive typed_table (K T : Type) : Type := a_typed_table.
+Inductive patterns (T : Type) : Type := a_pattern.
 
 (** Patterns **)
 Inductive RPattern : Type :=
@@ -13,18 +15,33 @@ Inductive RPattern : Type :=
 | RExact {T : Type} (value : T).
 
 (** Actions **)
-Definition function (f : Type)   : Type := f.
-Definition id       (T : Type)   : Type := T.
-Definition store    {K V : Type} (t : table K V) : Type := V.
+Definition function  (f : Type)   : Type := f.
+Definition id        (T : Type)   : Type := T.
+Definition associate {K : Type} (t : table K) (key : K) : Type.
+exact unit.
+Qed.
+Definition store     (K : Type) (t : table K) : Type := K.
 
 (** Commands **)
-Inductive Command :=
-| Patterns (T : Type)
-| Call (T : Type)
-| App {T : Type} (app : T -> T -> T)
-| Abs (T : Type) {U : Type} (lam : T -> U -> U)
-| Var {T : Type} (var : nat -> T)
-| Table (K V : Type) (t : table K V).
+Inductive Command (T : Type) :=
+| Fail
+| Patterns (f : patterns T) (_ : Command T)
+| Call (f : Type) (_ : Command T)
+| App (app : T -> T -> T) (_ : Command T)
+| Abs (U : Type) (lam : U -> T -> T) (_ : Command T)
+| Var (var : nat -> T) (_ : Command T)
+| Table (K : Type) (t : table K) (ctor : K -> T) (_ : Command T)
+| TypedTable (K Ty : Type) (t : typed_table K Ty) (ctor : K -> T) (_ : Command T).
+
+Require Coq.FSets.FMapPositive.
+
+(** Tables Reification Specification **)
+Definition mk_var_map {K V T : Type} (_ : table K) (ctor : V -> T) : Type :=
+  FMapPositive.PositiveMap.t T.
+Definition mk_dvar_map {K V T : Type} {F : V -> Type}
+              (_ : typed_table K V)
+              (ctor : forall x : V, F x -> T) :=
+  FMapPositive.PositiveMap.t T.
 
 (** Suggested Notation **)
 (*
