examples/Simple/SimpleExt.v
@@ -1,0 +1,63 @@
+Require Import MirrorCore.syms.SymEnv.
+Require Import MirrorCore.syms.SymSum.
+Require McExamples.Simple.Simple.
+
+Definition func := sum Simple.func SymEnv.func.
+
+Instance RSym_func fs : SymI.RSym func :=
+  @SymSum.RSym_sum Simple.typ _ Simple.func SymEnv.func _
+                   (@SymEnv.RSym_func Simple.typ _ fs).
+
+Require Import MirrorCore.Reify.Reify.
+Require Import MirrorCore.Lambda.ExprCore.
+
+(** Declare patterns **)
+Reify Declare Patterns patterns_simple_typ := Simple.typ.
+Reify Declare Patterns patterns_simple := (expr Simple.typ func).
+
+Reify Declare Syntax reify_simple_typ :=
+{ (@Patterns _ patterns_simple_typ (@Fail Simple.typ)) }.
+
+Reify Declare Typed Table table_terms : BinNums.positive => reify_simple_typ.
+
+Let typ := Simple.typ.
+Let other x := @Inj typ func (inr x).
+Print Patterns.TypedTable.
+
+(** Declare syntax **)
+Reify Declare Syntax reify_simple :=
+{ (@Patterns.Patterns _ patterns_simple
+  (@Patterns.App _ (@ExprCore.App typ func)
+  (@Patterns.Abs (expr typ func) reify_simple_typ (@ExprCore.Abs typ func)
+  (@Patterns.Var (expr typ func) (@ExprCore.Var typ func)
+  (@Patterns.TypedTable (expr typ func) BinNums.positive reify_simple_typ table_terms other
+  (@Patterns.Fail (expr typ func)))))))
+}.
+
+Reify Pattern patterns_simple_typ += (@RExact _ nat)  => Simple.tyNat.
+Reify Pattern patterns_simple_typ += (@RExact _ bool) => Simple.tyBool.
+Reify Pattern patterns_simple_typ += (@RExact _ Prop) => Simple.tyProp.
+Reify Pattern patterns_simple_typ += (@RImpl (@RGet 0 RIgnore) (@RGet 1 RIgnore)) => (fun (a b : function reify_simple_typ) => Simple.tyArr a b).
+
+Reify Pattern patterns_simple += (@RGet 0 RConst) => (fun (n : id nat) => @Inj typ func (inl (Simple.N n))).
+Reify Pattern patterns_simple += (RApp (RApp (@RExact _ plus) (RGet 0 RIgnore)) (RGet 1 RIgnore)) => (fun (a b : function reify_simple) => App (App (Inj (inl Simple.Plus)) a) b).
+Reify Pattern patterns_simple += (RApp (RApp (@RExact _ NPeano.ltb) (RGet 0 RIgnore)) (RGet 1 RIgnore)) => (fun (a b : function reify_simple) => App (App (Inj (inl Simple.Lt)) a) b).
+Reify Pattern patterns_simple += (RApp (RApp (RApp (@RExact _ (@eq)) (RGet 0 RIgnore)) (RGet 1 RIgnore)) (RGet 2 RIgnore)) => (fun (t : function reify_simple_typ) (a b : function reify_simple) => App (App (Inj (inl (Simple.Eq t))) a) b).
+
+Ltac reify_typ trm :=
+  let k e :=
+      refine e
+  in
+  reify_expr reify_simple_typ k [ True ] [ trm ].
+
+Ltac reify trm :=
+  let k e :=
+      refine e
+  in
+  reify_expr reify_simple k [ True ] [ trm ].
+
+Definition test_1 : expr typ func.
+  pose (x := 0).
+  reify (0 = x).
+Defined.
+Print test_1.
